fixed notation bug and some unification stuff

LeanLambdaLibMathlib/LambdaLib/unification.lean
@@ -9,17 +9,20 @@ open QuotTerm
 in this file, i'll define the actual unification tactic
 -/
 
+macro "normalize" : tactic => `(tactic|
+  simp [lift_app, lift_lam, lift_var, lift_const, subst_app, subst_lam, subst_var,
+      liftLiftMulti, substLiftMulti, subst_const, liftMultiZero, beta] at *
+)
+
 macro "lambda_solve" : tactic => `(tactic|
   repeat ( first
-    | simp [lift_app, lift_lam, lift_var, lift_const, subst_app, subst_lam, subst_var,
-      liftLiftMulti, substLiftMulti, subst_const, liftMultiZero, beta,
-      lam_body_rw, const_inj_rw, var_inj_rw, var_not_const_rw, var_not_const_rw2] at *
+    | normalize
+    | simp [lam_body_rw, const_inj_rw, var_inj_rw, var_not_const_rw, var_not_const_rw2] at *
     | simp (disch := repeat constructor) [app_fact_rw, app_ne_const_rw, app_ne_var_rw] at *
     | fail_if_no_progress subst_vars -- TODO: maybe only have this go on equations of type QTerm
   )
 )
 
--- for example, we want this to work:
 example (t1 t2 : QTerm)
   (H : < (λ x. x) {t1} > = <λ x. x>)
   : <{t1} {t2}> = t2 := by
@@ -31,30 +34,54 @@ example (H : <λ x. A> = <λ x. B>) : False := by
 example (H : <λ x. A> = <λ x. x>) : False := by
   lambda_solve
 
-/-
-there are two more cases i need unification to solve
-1) deriving contradiction from applications with different var or consts on left being equal
-x t1 = y t2 -> False,     A t1 = B t2 t3 -> False,  A t1 = x t2 -> False, .....
-2) equality of children of application from equality of applications with same head and arity
-x t1 t2 = y t1' t2' -> t1 = t1', t2 = t2'
-
-see https://leanprover-community.github.io/extras/simp.html
-simp can discharge premises to decide. maybe i can make eta reduce by making the lift property
-decidable?
-
-the idea would be make a property (incompatible : QTerm -> QTerm -> Prop) which holds when the terms
-are apps with different l.h.s. or arities, and then
-a theorem ((incompat t1 t2) → (t1 = t2) = False)
-then it can simp by that
-
-see: https://lean-lang.org/theorem_proving_in_lean4/Type-Classes/#decidable-propositions
--/
-
-#check app_ne_var
-#check app_ne_const
-#check app_fact
-
--- so i need to make simp able to try to prove QNeutral using (repeat constructor) maybe?
-
 example (t1 t2 : QTerm) (H : <A {t1} > = <A {t2} >) : t1 = t2 := by
   lambda_solve
+
+example (H : <A B> = <A C>) : False := by
+  lambda_solve
+
+abbrev zero := <λ s z. z>
+abbrev succ := <λ n. λ s z. s (n s z)>
+abbrev plus := <λ a b. a {succ} (b {succ} {zero})>
+abbrev mult := <λ a b. a (b {succ}) {zero}>
+
+abbrev one := <{succ} {zero}>
+abbrev two := <{succ} ({succ} {zero})>
+abbrev four := <{succ} ({succ} {two})>
+
+abbrev two2 := <λ s z. s (s z)>
+abbrev four2 := <λ s z. s (s (s (s z)))>
+
+example : <{plus} {zero} {zero}> = zero := by
+  lambda_solve
+
+example : <{plus} {one} {one}> = two := by
+  unfold plus one two succ zero
+  lambda_solve
+
+example : <{plus} {two} {two}> = four := by
+  unfold plus two succ zero four
+  lambda_solve
+
+example : <{plus} {two2} {two2}> = four2 := by
+  lambda_solve
+  --
+
+example : <{mult} {zero} {zero}> = zero := by
+  lambda_solve
+
+example : <{mult} {one} {one}> = one := by
+  unfold mult succ one
+  lambda_solve
+  --
+
+example : <{mult} {two} {two}> = four := by
+  unfold two four mult succ zero
+  lambda_solve
+  --
+
+-- need rewrites for liftMulti
+example : <λ x. {plus} {zero} {zero}> = <λ x. zero> := by
+  unfold plus zero succ
+  lambda_solve
+  --
